removed Map from docu

src/HOL/Data_Structures/Trie_Map.thy
@@ -6,14 +6,31 @@ imports
   Trie_Fun
 begin
 
-text \<open>An implementation of tries based on maps implemented by red-black trees.
-Works for any kind of search tree.\<close>
+text \<open>An implementation of tries for an arbitrary alphabet \<open>'a\<close> where
+the mapping from an element of type \<open>'a\<close> to the sub-trie is implemented by a binary search tree.
+Although this implementation uses maps implemented by red-black trees it works for any
+implementation of maps.
 
-text \<open>Implementation of map:\<close>
+This is an implementation of the ``ternary search trees'' by Bentley and Sedgewick
+[SODA 1997, Dr. Dobbs 1998]. The name derives from the fact that a node in the BST can now
+be drawn to have 3 children, where the middle child is the sub-trie that the node maps
+its key to. Hence the name \<open>trie3\<close>.
 
-type_synonym 'a mapi = "'a rbt"
+Example from @{url "https://en.wikipedia.org/wiki/Ternary_search_tree#Description"}:
 
-datatype 'a trie_map = Nd bool "('a * 'a trie_map) mapi"
+          c
+        / | \
+       a  u  h
+       |  |  | \
+       t. t  e. u
+     /  / |   / |
+    s. p. e. i. s.
+
+Characters with a dot are final.
+Thus the tree represents the set of strings "cute","cup","at","as","he","us" and "i".
+\<close>
+
+datatype 'a trie3 = Nd3 bool "('a * 'a trie3) rbt"
 
 text \<open>In principle one should be able to given an implementation of tries
 once and for all for any map implementation and not just for a specific one (RBT) as done here.
@@ -21,89 +38,90 @@ But because the map (@{typ "'a rbt"}) is used in a datatype, the HOL type system
 
 However, the development below works verbatim for any map implementation, eg \<open>Tree_Map\<close>,
 and not just \<open>RBT_Map\<close>, except for the termination lemma \<open>lookup_size\<close>.\<close>
+
 term size_tree
 lemma lookup_size[termination_simp]:
-  fixes t :: "('a::linorder * 'a trie_map) rbt"
+  fixes t :: "('a::linorder * 'a trie3) rbt"
   shows "lookup t a = Some b \<Longrightarrow> size b < Suc (size_tree (\<lambda>ab. Suc(Suc (size (snd(fst ab))))) t)"
 apply(induction t a rule: lookup.induct)
 apply(auto split: if_splits)
 done
 
 
-definition empty :: "'a trie_map" where
-[simp]: "empty = Nd False Leaf"
+definition empty3 :: "'a trie3" where
+[simp]: "empty3 = Nd3 False Leaf"
 
-fun isin :: "('a::linorder) trie_map \<Rightarrow> 'a list \<Rightarrow> bool" where
-"isin (Nd b m) [] = b" |
-"isin (Nd b m) (x # xs) = (case lookup m x of None \<Rightarrow> False | Some t \<Rightarrow> isin t xs)"
+fun isin3 :: "('a::linorder) trie3 \<Rightarrow> 'a list \<Rightarrow> bool" where
+"isin3 (Nd3 b m) [] = b" |
+"isin3 (Nd3 b m) (x # xs) = (case lookup m x of None \<Rightarrow> False | Some t \<Rightarrow> isin3 t xs)"
 
-fun insert :: "('a::linorder) list \<Rightarrow> 'a trie_map \<Rightarrow> 'a trie_map" where
-"insert [] (Nd b m) = Nd True m" |
-"insert (x#xs) (Nd b m) =
-  Nd b (update x (insert xs (case lookup m x of None \<Rightarrow> empty | Some t \<Rightarrow> t)) m)"
+fun insert3 :: "('a::linorder) list \<Rightarrow> 'a trie3 \<Rightarrow> 'a trie3" where
+"insert3 [] (Nd3 b m) = Nd3 True m" |
+"insert3 (x#xs) (Nd3 b m) =
+  Nd3 b (update x (insert3 xs (case lookup m x of None \<Rightarrow> empty3 | Some t \<Rightarrow> t)) m)"
 
-fun delete :: "('a::linorder) list \<Rightarrow> 'a trie_map \<Rightarrow> 'a trie_map" where
-"delete [] (Nd b m) = Nd False m" |
-"delete (x#xs) (Nd b m) = Nd b
+fun delete3 :: "('a::linorder) list \<Rightarrow> 'a trie3 \<Rightarrow> 'a trie3" where
+"delete3 [] (Nd3 b m) = Nd3 False m" |
+"delete3 (x#xs) (Nd3 b m) = Nd3 b
    (case lookup m x of
       None \<Rightarrow> m |
-      Some t \<Rightarrow> update x (delete xs t) m)"
+      Some t \<Rightarrow> update x (delete3 xs t) m)"
 
 
 subsection "Correctness"
 
-text \<open>Proof by stepwise refinement. First abstract to type @{typ "'a trie"}.\<close>
+text \<open>Proof by stepwise refinement. First abs3tract to type @{typ "'a trie"}.\<close>
 
-fun abs :: "'a::linorder trie_map \<Rightarrow> 'a trie" where
-"abs (Nd b t) = Trie_Fun.Nd b (\<lambda>a. map_option abs (lookup t a))"
+fun abs3 :: "'a::linorder trie3 \<Rightarrow> 'a trie" where
+"abs3 (Nd3 b t) = Nd b (\<lambda>a. map_option abs3 (lookup t a))"
 
-fun invar :: "('a::linorder)trie_map \<Rightarrow> bool" where
-"invar (Nd b m) = (M.invar m \<and> (\<forall>a t. lookup m a = Some t \<longrightarrow> invar t))"
+fun invar3 :: "('a::linorder)trie3 \<Rightarrow> bool" where
+"invar3 (Nd3 b m) = (M.invar m \<and> (\<forall>a t. lookup m a = Some t \<longrightarrow> invar3 t))"
 
-lemma isin_abs: "isin t xs = Trie_Fun.isin (abs t) xs"
-apply(induction t xs rule: isin.induct)
+lemma isin_abs3: "isin3 t xs = isin (abs3 t) xs"
+apply(induction t xs rule: isin3.induct)
 apply(auto split: option.split)
 done
 
-lemma abs_insert: "invar t \<Longrightarrow> abs(insert xs t) = Trie_Fun.insert xs (abs t)"
-apply(induction xs t rule: insert.induct)
+lemma abs3_insert3: "invar3 t \<Longrightarrow> abs3(insert3 xs t) = insert xs (abs3 t)"
+apply(induction xs t rule: insert3.induct)
 apply(auto simp: M.map_specs RBT_Set.empty_def[symmetric] split: option.split)
 done
 
-lemma abs_delete: "invar t \<Longrightarrow> abs(delete xs t) = Trie_Fun.delete xs (abs t)"
-apply(induction xs t rule: delete.induct)
+lemma abs3_delete3: "invar3 t \<Longrightarrow> abs3(delete3 xs t) = delete xs (abs3 t)"
+apply(induction xs t rule: delete3.induct)
 apply(auto simp: M.map_specs split: option.split)
 done
 
-lemma invar_insert: "invar t \<Longrightarrow> invar (insert xs t)"
-apply(induction xs t rule: insert.induct)
+lemma invar3_insert3: "invar3 t \<Longrightarrow> invar3 (insert3 xs t)"
+apply(induction xs t rule: insert3.induct)
 apply(auto simp: M.map_specs RBT_Set.empty_def[symmetric] split: option.split)
 done
 
-lemma invar_delete: "invar t \<Longrightarrow> invar (delete xs t)"
-apply(induction xs t rule: delete.induct)
+lemma invar3_delete3: "invar3 t \<Longrightarrow> invar3 (delete3 xs t)"
+apply(induction xs t rule: delete3.induct)
 apply(auto simp: M.map_specs split: option.split)
 done
 
 text \<open>Overall correctness w.r.t. the \<open>Set\<close> ADT:\<close>
 
 interpretation S2: Set
-where empty = empty and isin = isin and insert = insert and delete = delete
-and set = "set o abs" and invar = invar
+where empty = empty3 and isin = isin3 and insert = insert3 and delete = delete3
+and set = "set o abs3" and invar = invar3
 proof (standard, goal_cases)
   case 1 show ?case by (simp add: isin_case split: list.split)
 next
-  case 2 thus ?case by (simp add: isin_abs)
+  case 2 thus ?case by (simp add: isin_abs3)
 next
-  case 3 thus ?case by (simp add: set_insert abs_insert del: set_def)
+  case 3 thus ?case by (simp add: set_insert abs3_insert3 del: set_def)
 next
-  case 4 thus ?case by (simp add: set_delete abs_delete del: set_def)
+  case 4 thus ?case by (simp add: set_delete abs3_delete3 del: set_def)
 next
   case 5 thus ?case by (simp add: M.map_specs RBT_Set.empty_def[symmetric])
 next
-  case 6 thus ?case by (simp add: invar_insert)
+  case 6 thus ?case by (simp add: invar3_insert3)
 next
-  case 7 thus ?case by (simp add: invar_delete)
+  case 7 thus ?case by (simp add: invar3_delete3)
 qed
 
 
